commit

AP/AP/FreshA.lean
@@ -2,6 +2,17 @@ import AP.AP.King
 
 namespace AP
 
+class AStrat.Fresh (a : AStrat) (s : State) extends wf : a.WF where
+  h₁ : ∀ {d : DStrat} [d.WF] {s₁ s₂ : State} [AState s₁] [AState s₂]
+    {k n : ℕ}, k < n → sys.simulate (Strat.f ⟨a, d⟩) s k = (s₁, 0) →
+    sys.simulate (Strat.f ⟨a, d⟩) s n = (s₂, 0) →
+    sys.hasTr s₂ → s.pw < (a.f s₂).dist s₁.aPos
+
+-- open Classical in noncomputable
+-- def aFresh : AStrat :=
+--   .mk # λ s => choose? # λ p => ∃ s', sys.tr s p = some s' ∧
+--   s'.aHws ∧ ∀ p₁ s₁, sys.tr s p₁ = some s₁ → s₁.aHws → s'.taken ⊆ s₁.taken
+
 theorem State.aHws_of_taken_subset {s s'} [hs : sys.WF s] [hs' : sys.WF s']
 (h₁ : s.aHws) (hpw : s.pw = s'.pw) (h₂ : s.aTurn = s'.aTurn) (h₃ : s.aPos = s'.aPos)
 (h₄ : s'.taken ⊆ s.taken) : s'.aHws := by
@@ -58,3 +69,70 @@ theorem State.aHws_of_taken_subset {s s'} [hs : sys.WF s] [hs' : sys.WF s']
       rintro (rfl | H₆) <;> right
       · exact hp
       exact H₃ p₁ H₆
+
+#check 0 #exit
+
+instance : aFresh.WF := by unfold aFresh; infer_instance
+
+-- #check 0 #exit
+
+theorem exi_tr_aHws_min_taken_of_aHws {s} [hs : sys.WF s] (h : s.aHws) :
+∃ p s', sys.tr s p = some s' ∧ s'.aHws ∧ ∀ p₁ s₁,
+sys.tr s p₁ = some s₁ → s₁.aHws → s'.taken ⊆ s₁.taken := by
+  sorry
+
+-- #check 0 #exit
+
+theorem aFresh_cnd_of_aHws {s} [hs : sys.WF s] (h : s.aHws) :
+∃ s', sys.tr s (aFresh.f s) = some s' ∧ s'.aHws ∧ ∀ p₁ s₁,
+sys.tr s p₁ = some s₁ → s₁.aHws → s'.taken ⊆ s₁.taken := by
+  have h₃ := exi_tr_aHws_min_taken_of_aHws h
+  have h₄ := Classical.epsilon_spec h₃
+  generalize hp : (Classical.epsilon # λ p => ∃ s', sys.tr s p = some s' ∧ s'.aHws ∧
+    ∀ p₁ s₁, sys.tr s p₁ = some s₁ → s₁.aHws → s'.taken ⊆ s₁.taken) = p at h₄
+  obtain ⟨s₁, h₄, h₅, h₆⟩ := h₄
+  simpa [-AState.tr_eq_some_iff, aFresh, choose?_eq_ite, h₃, hp,
+    sys.validTr_of_eq_some h₄, h₄, h₅]
+
+theorem aFresh_cnd_of_aHws_and_tr {s s'} [hs : sys.WF s] (h₁ : s.aHws)
+(h₂ : sys.tr s (aFresh.f s) = some s') : s'.aHws ∧ ∀ p₁ s₁,
+sys.tr s p₁ = some s₁ → s₁.aHws → s'.taken ⊆ s₁.taken := by
+  obtain ⟨s₁, h₃, h₄⟩ := aFresh_cnd_of_aHws h₁
+  simp [h₂] at h₃; subst h₃; exact h₄
+
+theorem aHws_of_tr_aFresh {s s'} [hs : sys.WF s]
+(h₁ : s.aHws) (h₂ : sys.tr s (aFresh.f s) = some s') : s'.aHws :=
+  aFresh_cnd_of_aHws_and_tr h₁ h₂ |>.1
+
+theorem aHws_of_simulate_aFresh {s} [hs : sys.WF s] {d : DStrat} {n}
+(h : s.aHws) : sys.simulate (Strat.f ⟨aFresh, d⟩) s n |>.1.aHws := by
+  induction n generalizing s; exact h
+  nm n ih; simp; split; exact h; nm x s' h₁
+  clear x; replace hs := s.aState_or_dState
+  rcases hs with hs | hs
+  · have hs' := DState.of_tr h₁; apply ih
+    simp [-AState.tr_eq_some_iff] at h₁
+    exact aHws_of_tr_aFresh h h₁
+  · have hs' := AState.of_tr h₁
+    apply ih; exact DState.aHws_of_tr h₁ h
+
+theorem aHws_of_simulate_aFresh_eq {s r} [hs : sys.WF s] {d : DStrat} {n}
+(h₁ : s.aHws) (h₂ : sys.simulate (Strat.f ⟨aFresh, d⟩) s n = r) : r.1.aHws := by
+  subst h₂; exact aHws_of_simulate_aFresh h₁
+
+-- #check 0 #exit
+
+theorem fresh_aFresh_of_aHws {s} [hs : sys.WF s]
+(h : s.aHws) : aFresh.Fresh s := by
+  constructor
+  intro d hd s₁ s₂ hs₁ hs₂ k n hk h₁ h₂ h₃
+  by_contra! h₄
+  apply aFresh.validTr at h₃
+  obtain ⟨s₃, h₃⟩ := h₃
+  have H₁ := aHws_of_simulate_aFresh_eq h h₁
+  have H₂ := aHws_of_simulate_aFresh_eq h h₂
+  dsimp at H₁ H₂
+  obtain ⟨H₃, H₄⟩ := aFresh_cnd_of_aHws_and_tr H₂ h₃
+  by_cases h₅ : aFresh.f s₂ = s₁.aPos
+  · sorry
+  sorry
